feat: closed_at_neutral

CollapsingTowers/TwoLevel/Neutral.lean
@@ -1,9 +1,10 @@
 
 import CollapsingTowers.TwoLevel.Basic
+import CollapsingTowers.TwoLevel.OpenClose
 @[simp]
 def neutral (x : ℕ) : Expr -> Prop
   | .bvar _ => true
-  | .fvar y => y ≠ x
+  | .fvar _ => false
   | .lam₁ e => neutral x e
   | .lam₂ e => neutral x e
   | .app₁ f arg => neutral x f ∧ neutral x arg
@@ -12,11 +13,11 @@ def neutral (x : ℕ) : Expr -> Prop
   | .lit₂ n => neutral x n
   | .plus₁ l r => neutral x l ∧ neutral x r
   | .plus₂ l r => neutral x l ∧ neutral x r
-  | .code _ => true
-  | .reflect _ => true
+  | .code e => closed_at e x
+  | .reflect e => closed_at e x
   | .lam𝕔 e => neutral x e
   | .lets b e => neutral x b ∧ neutral x e
-  | .let𝕔 _ e => neutral x e
+  | .let𝕔 b e => closed_at b x ∧ neutral x e
 
 @[simp]
 def neutral_db (i : ℕ) : Expr -> Prop
@@ -57,3 +58,30 @@ def wf_expr : Expr -> Prop
   | .lam𝕔 e => neutral_lc e ∧ wf_expr e
   | .lets b e => wf_expr b ∧ wf_expr e
   | .let𝕔 b e => wf_expr b ∧ neutral_lc e ∧ wf_expr e
+
+theorem closed_at_neutral : ∀ e, closed_at e 0 -> neutral 0 e :=
+  by
+  intros e Hclose
+  induction e with
+  | bvar| lit₁ => simp
+  | code| reflect => apply Hclose
+  | fvar => nomatch Hclose
+  | lam₁ _ IH
+  | lam₂ _ IH
+  | lit₂ _ IH
+  | lam𝕔 _ IH => simp at *; apply IH; apply Hclose
+  | app₁ _ _ IH₀ IH₁
+  | app₂ _ _ IH₀ IH₁
+  | plus₁ _ _ IH₀ IH₁
+  | plus₂ _ _ IH₀ IH₁ =>
+    simp; constructor
+    apply IH₀; apply Hclose.left
+    apply IH₁; apply Hclose.right
+  | lets _ _ IHb IHe =>
+    simp; constructor
+    apply IHb; apply Hclose.left
+    apply IHe; apply Hclose.right
+  | let𝕔 _ _ _ IHe =>
+    simp; constructor
+    apply Hclose.left
+    apply IHe; apply Hclose.right
